\documentclass{article}

\usepackage{amsmath,amssymb}
\usepackage{tikz}
\usepackage{xcolor}
\usepackage[left=2.1cm,right=3.1cm,bottom=3cm,footskip=0.75cm,headsep=0.5cm]{geometry}
\usepackage{enumerate}
\usepackage{enumitem}
\usepackage{marvosym}
\usepackage{tabularx}
\usepackage{xcolor}
\usepackage{colortbl}

\usepackage[utf8]{inputenc}

\renewcommand*{\arraystretch}{1.4}

\newcolumntype{L}[1]{>{\raggedright\arraybackslash}p{#1}}
\newcolumntype{R}[1]{>{\raggedleft\arraybackslash}p{#1}}
\newcolumntype{C}[1]{>{\centering\let\newline\\\arraybackslash\hspace{0pt}}m{#1}}

\title{\textbf{Einführung in die Informatik, Übung 12}}
\author{\textsc{Henry Haustein}}
\date{}

\begin{document}
	\maketitle
	
	\section*{Aufgabe 12.1}
	
	\begin{enumerate}[label=(\alph*)]
		\item alle Modelle von $\Gamma$ finden:
		\begin{center}
			\begin{tabular}{ccc||c|c|c}
				$p$ & $q$ & $r$ & $p\Rightarrow q$ & $r\lor p$ & $\neg q\lor r$ \\
				\hline
				0 & 0 & 0 & 1 & 0 & 1 \\
				0 & 0 & 1 & \textcolor{red}{1} & \textcolor{red}{1} & \textcolor{red}{1} \\
				0 & 1 & 0 & 1 & 0 & 0 \\
				0 & 1 & 1 & \textcolor{red}{1} & \textcolor{red}{1} & \textcolor{red}{1} \\
				1 & 0 & 0 & 0 & 1 & 1 \\
				1 & 0 & 1 & 0 & 1 & 1 \\
				1 & 1 & 0 & 1 & 1 & 0 \\
				1 & 1 & 1 & \textcolor{red}{1} & \textcolor{red}{1} & \textcolor{red}{1} \\
			\end{tabular}
		\end{center}
		3 Modelle erfüllen $\Gamma$
		\item $\Gamma\models (\neg p\lor r)$, denn
		\begin{center}
			\begin{tabular}{ccc||c}
				$p$ & $q$ & $r$ & $\neg p\lor r$ \\
				\hline
				0 & 0 & 1 & 1 \\
				0 & 1 & 1 & 1 \\
				1 & 1 & 1 & 1 \\
			\end{tabular}
		\end{center}
		\item $\Gamma\not\models (\neg q\land r)$, denn
		\begin{center}
			\begin{tabular}{ccc||c}
				$p$ & $q$ & $r$ & $\neg q\land r$ \\
				\hline
				0 & 0 & 1 & 1 \\
				0 & 1 & 1 & 0 \\
				1 & 1 & 1 & 0 \\
			\end{tabular}
		\end{center}
		\item $\Gamma\models (q\lor r)$, denn
		\begin{center}
			\begin{tabular}{ccc||c}
				$p$ & $q$ & $r$ & $q\lor r$ \\
				\hline
				0 & 0 & 1 & 1 \\
				0 & 1 & 1 & 1 \\
				1 & 1 & 1 & 1 \\
			\end{tabular}
		\end{center}
	\end{enumerate}
	
	\section*{Aufgabe 12.2}
	\begin{enumerate}[label=(\alph*)]
		\item siehe Tabelle
		\begin{center}
			\begin{tabular}{cc||c|c|c}
				$\phi$ & $\psi$ & $\phi\lor\psi$ & $\phi\land(\phi\lor\psi)$ & $\phi\land(\phi\lor\psi)\equiv\phi$ \\
				\hline
				0 & 0 & 0 & 0 & 1 \\
				0 & 1 & 1 & 0 & 1 \\
				1 & 0 & 1 & 1 & 1 \\
				1 & 1 & 1 & 1 & 1 \\
			\end{tabular}
		\end{center}
		\item siehe Tabelle
		\begin{center}
			\begin{tabular}{ccc||c|c|c|c|c|c}
				$\phi$ & $\psi$ & $\pi$ & $\psi\lor\pi$ & $\phi\land(\psi\lor\pi)$ & $\phi\land\psi$ & $\phi\land\pi$ & $(\phi\land\psi)\lor(\phi\land\pi)$ & $\phi\land(\psi\lor\pi)\equiv(\phi\land\psi)\lor(\phi\land\pi)$ \\
				\hline
				0 & 0 & 0 & 0 & 0 & 0 & 0 & 0 & 1 \\
				0 & 0 & 1 & 1 & 0 & 0 & 0 & 0 & 1 \\
				0 & 1 & 0 & 1 & 0 & 0 & 0 & 0 & 1 \\
				0 & 1 & 1 & 1 & 0 & 0 & 0 & 0 & 1 \\
				1 & 0 & 0 & 0 & 0 & 0 & 0 & 0 & 1 \\
				1 & 0 & 1 & 1 & 1 & 0 & 1 & 1 & 1 \\
				1 & 1 & 0 & 1 & 1 & 1 & 0 & 1 & 1 \\
				1 & 1 & 1 & 1 & 1 & 1 & 1 & 1 & 1
			\end{tabular}
		\end{center}
	\end{enumerate}

	\section*{Aufgabe 12.3}
	Ersetzungen:
	\begin{itemize}
		\item $a\lor b\equiv \neg\neg a\lor\neg\neg b\equiv\neg(\neg a\land\neg b)$
		\item $c\Leftrightarrow d\equiv (c\land d)\lor(\neg c\land\neg d) \equiv \neg(\neg (c\land d)\land\neg (\neg c\land\neg d))$
	\end{itemize}
	\begin{align}
		\phi &= \neg(((\neg p\lor q)\lor(p\Leftrightarrow\neg q))\textcolor{red}{\,\lor\,}\neg(r\land(s\lor r))) \notag \\
		&= \neg(\neg(\neg ((\neg p\lor q)\lor(p\Leftrightarrow\neg q))\land\neg(\neg(r\land(s\textcolor{red}{\,\lor\,} r))))) \notag \\
		&= \neg(\neg(\neg ((\neg p\lor q)\textcolor{red}{\,\lor\,}(p\Leftrightarrow\neg q))\land\neg(\neg(r\land(\neg(\neg s\land\neg r)))))) \notag \\
		&= \neg(\neg(\neg (\neg(\neg (\neg p\textcolor{red}{\,\lor\,} q)\land\neg (p\Leftrightarrow\neg q)))\land\neg(\neg(r\land(\neg(\neg s\land\neg r)))))) \notag \\
		&= \neg(\neg(\neg (\neg(\neg (\neg(\neg (\neg p)\land\neg q))\land\neg (p\textcolor{red}{\,\Leftrightarrow\,}\neg q)))\land\neg(\neg(r\land(\neg(\neg s\land\neg r)))))) \notag \\
		&= \neg(\neg(\neg (\neg(\neg (\neg(\neg (\neg p)\land\neg q))\land\neg (\neg(\neg (p\land \neg q)\land\neg (\neg p\land\neg \neg q)))))\land\neg(\neg(r\land(\neg(\neg s\land\neg r)))))) \notag
	\end{align}
	
	\section*{Aufgabe 12.4}
	\begin{enumerate}[label=(\alph*)]
		\item siehe Tabelle

	\end{enumerate}

	\section*{Aufgabe 12.5}

\end{document}